Sorting/SelectionSort.v
@@ -10,25 +10,13 @@ Set Implicit Arguments.
 Function ss (A : LinDec) (l : list A) {measure length l} : list A :=
 match l with
     | [] => []
-    | h :: t => let m := min_dflt A h t in m :: ss A (remove_once m l)
+    | h :: t => let m := min_dflt A h t in m :: ss A (removeFirst m l)
 end.
-Proof. intros. apply remove_once_min_lengthOrder. Defined.
+Proof. intros. apply removeFirst_min_lengthOrder. Defined.
 
-Function minmax (A : LinDec) (min : A) (max : A) (l : list A) : A * A :=
-match l with
-    | [] => (min, max)
-    | h :: t =>
-        if h <=? min
-        then minmax A h max t
-        else
-          if max <=? h
-          then minmax A min h t
-          else minmax A min max t
-end.
-
-Lemma remove_once_In' :
+Lemma removeFirst_In' :
   forall (A : LinDec) (x h : A) (t : list A),
-    In x t -> x <> h -> In x (remove_once h t).
+    In x t -> x <> h -> In x (removeFirst h t).
 Proof.
   induction t as [| h' t']; cbn; intuition dec.
 Qed.
