Sorting/SelectionSort2.v
@@ -19,7 +19,7 @@ Function ss (A : LinDec) (l : list A) {measure length l} : list A :=
 match min l with
     | None => []
     | Some m =>
-        m :: ss A (remove_once m l)
+        m :: ss A (removeFirst m l)
 end.
 Proof.
   intros. functional induction @min A l; inv teq; cbn; dec.
@@ -38,9 +38,9 @@ Proof.
       exists (h :: l1), l2. cbn. reflexivity.
 Qed.
 
-Lemma remove_once_middle :
+Lemma removeFirst_middle :
   forall (A : LinDec) (m : A) (l1 l2 : list A),
-    perm A (l1 ++ l2) (remove_once m (l1 ++ m :: l2)).
+    perm A (l1 ++ l2) (removeFirst m (l1 ++ m :: l2)).
 Proof.
   induction l1 as [| h t]; cbn; intros; dec.
 Qed.
@@ -53,7 +53,7 @@ Proof.
     destruct (min_present _ _ e) as (l1 & l2 & Heq). subst.
       eapply perm_trans.
         apply perm_front.
-        apply perm_cons. rewrite <- IHl0. apply remove_once_middle.
+        apply perm_cons. rewrite <- IHl0. apply removeFirst_middle.
 Qed.
 
 Lemma ss_In :
@@ -75,9 +75,9 @@ Proof.
     inv H. dec.
 Qed.
 
-Lemma remove_once_min_In :
+Lemma removeFirst_min_In :
   forall (A : LinDec) (x m : A) (l : list A),
-    In x l -> x <> m -> min l = Some m -> In x (remove_once m l).
+    In x l -> x <> m -> min l = Some m -> In x (removeFirst m l).
 Proof.
   intros. functional induction min l; inv H1.
     inv H. destruct t.
@@ -87,9 +87,9 @@ Proof.
     cbn. inv H; dec.
 Qed.
 
-Lemma remove_once_In :
+Lemma removeFirst_In :
   forall (A : LinDec) (x m : A) (l : list A),
-    In x (remove_once m l) -> In x l.
+    In x (removeFirst m l) -> In x l.
 Proof.
   induction l as [| h t]; cbn; intros.
     assumption.
@@ -101,9 +101,9 @@ Theorem ss_sorted :
 Proof.
   intros. functional induction ss A l.
     constructor.
-    destruct (ss A (remove_once m l)) eqn: Heq; constructor.
+    destruct (ss A (removeFirst m l)) eqn: Heq; constructor.
       apply min_spec with l.
-        apply remove_once_In with m. rewrite <- ss_In, Heq. left. auto.
+        apply removeFirst_In with m. rewrite <- ss_In, Heq. left. auto.
         assumption.
       assumption.
 Qed.
@@ -114,3 +114,150 @@ Instance Sort_ss (A : LinDec) : Sort A :=
     sort_sorted := ss_sorted A;
     sort_perm := ss_perm A
 }.
+
+(** Selection sort on steroids *)
+
+Function mins {A : LinDec} (l : list A) : list A :=
+match l with
+    | [] => []
+    | h :: t =>
+        let l' := mins t in
+        match l' with
+            | [] => [h]
+            | m :: ms =>
+                if h =? m
+                then h :: l'
+                else if h <=? m
+                then [h]
+                else l'
+        end
+end.
+
+(*Fixpoint removeAll
+  {A : Type} (p : A -> bool) (l : list A) : list A :=
+match l with
+    | [] => []
+    | h :: t => if p h then removeAll p t else h :: remove_all p t
+end.
+
+Lemma length_removeAll :
+  forall (A : Type) (p : A -> bool) ( *)
+
+Lemma ss'_aux :
+  forall (A : LinDec) (l : list A) (h : A) (t : list A),
+    mins l = h :: t ->
+      length (filter (fun x : A => negb (x =? h)) l) < length l.
+Proof.
+  induction l as [| h' t']; cbn in *; intros.
+    inv H.
+    destruct (mins t'); dec; inv H.
+      1-3: apply le_n_S; apply filter_length.
+      apply lt_n_S. apply IHt' with t. reflexivity.
+Qed.
+
+Function ss'
+  {A : LinDec} (l : list A) {measure length l} : list A :=
+match mins l with
+    | [] => []
+    | h :: t => (h :: t) ++ ss' (filter (fun x => negb (x =? h)) l)
+end.
+Proof.
+  apply ss'_aux.
+Defined.
+
+Function ss''
+  {A : LinDec} (l : list A) {measure length l} : list A :=
+match min l with
+    | None => []
+    | Some m =>
+        filter (fun x => x =? m) l ++
+        ss'' (filter (fun x => negb (x =? m)) l)
+end.
+Proof.
+  intros. functional induction min l; cbn; inv teq; dec.
+    1-3: apply le_n_S, filter_length.
+    apply lt_n_S, IHo. assumption.
+Defined.
+
+Function ss_bifilter
+  {A : LinDec} (l : list A) {measure length l} : list A :=
+match min l with
+    | None => []
+    | Some m =>
+        let
+          (l1, l2) := bifilter (fun x => x =? m) l
+        in
+          l1 ++ ss_bifilter l2
+end.
+Proof.
+  intros. functional induction min l; cbn in *; inv teq;
+  rewrite bifilter_spec in *; dec; inv teq0.
+    1-3: apply le_n_S, filter_length.
+    cbn. apply lt_n_S. eapply IHo; eauto. apply bifilter_spec.
+Defined.
+
+(** Da ultimate selection sort! *)
+
+Require Import TrichDec.
+
+Function mins'
+  {A : TrichDec} (l : list A) : list A * list A :=
+match l with
+    | [] => ([], [])
+    | h :: t =>
+        let
+          (mins, rest) := mins' t
+        in
+          match mins with
+              | [] => ([h], rest)
+              | m :: ms =>
+                  match h <?> m with
+                      | Lt => ([h], mins ++ rest)
+                      | Eq => (h :: mins, rest)
+                      | Gt => (mins, h :: rest)
+                  end
+          end
+end.
+
+Lemma mins'_nil :
+  forall (A : TrichDec) (l rest : list A),
+    mins' l = ([], rest) -> rest = [].
+Proof.
+  intros. functional induction mins' l; inv H.
+Qed.
+
+Lemma mins'_length :
+  forall (A : TrichDec) (l mins rest : list A),
+    mins' l = (mins, rest) -> length l = length mins + length rest.
+Proof.
+  intros. functional induction mins' l; inv H; cbn in *.
+    destruct t; cbn in e0.
+      inv e0.
+      destruct (mins' t), l.
+        inv e0.
+        destruct (c <?> c0); inv e0.
+    1-3: f_equal; rewrite (IHp _ _ e0), ?app_length; cbn; omega.
+Qed.
+
+Function ss_mins'
+  {A : TrichDec} (l : list A) {measure length l} : list A :=
+match mins' l with
+    | ([], _) => []
+    | (mins, rest) => mins ++ ss_mins' rest
+end.
+Proof.
+  intros. functional induction mins' l; inv teq; cbn in *.
+    apply mins'_nil in e0. subst. cbn. apply le_n_S, le_0_n.
+    all: apply mins'_length in e0; cbn in e0;
+      rewrite e0, ?app_length; omega.
+Defined.
+
+(*Time Compute ss natle (cycle 500 testl).
+Time Compute ss' natle (cycle 500 testl).
+Time Compute ss'' natle (cycle 500 testl).
+Time Compute ss_bifilter natle (cycle 500 testl).
+Time Compute ss_mins' natlt (cycle 500 testl).*)
+
+(** Time to prove something *)
+
+(*Class MinMaxRest *)
