Sorting/Sort_generalized.v
@@ -4,32 +4,32 @@ Require Export RCCBase.
 
 Require Export Sorting.Perm.
 
-Inductive sorted (A : LinDec) : list A -> Prop :=
-    | sorted0 : sorted A []
-    | sorted1 : forall x : A, sorted A [x]
+Inductive sorted {A : Type} (R : A -> A -> Prop) : list A -> Prop :=
+    | sorted0 : sorted R []
+    | sorted1 : forall x : A, sorted R [x]
     | sorted2 : forall (x y : A) (l : list A),
-        x ≤ y -> sorted A (y :: l) -> sorted A (x :: y :: l).
+        R x y -> sorted R (y :: l) -> sorted R (x :: y :: l).
 
 Hint Constructors sorted.
 
-Class Sort (A : LinDec) : Type :=
+Class Sort (A : Type) (R : A -> A -> Prop) : Type :=
 {
     sort :> list A -> list A;
     sort_sorted :
-      forall l : list A, sorted A (sort l);
+      forall l : list A, sorted R (sort l);
     sort_perm :
-      forall l : list A, perm A l (sort l);
+      forall l : list A, Permutation l (sort l);
 }.
 
 Coercion sort : Sort >-> Funclass.
 
-Class Partition (A : LinDec) : Type :=
+Class Partition (A : Type) (R : A -> A -> Prop) : Type :=
 {
     partition :> A -> list A -> list A * list A * list A;
     spec_lo :
       forall (pivot : A) (l lo eq hi : list A),
         partition pivot l = (lo, eq, hi) ->
-          forall x : A, In x lo -> x ≤ pivot;
+          forall x : A, In x lo -> R x pivot;
     spec_eq :
       forall (pivot : A) (l lo eq hi : list A),
         partition pivot l = (lo, eq, hi) ->
@@ -37,7 +37,7 @@ Class Partition (A : LinDec) : Type :=
     spec_hi :
       forall (pivot : A) (l lo eq hi : list A),
         partition pivot l = (lo, eq, hi) ->
-          forall x : A, In x hi -> pivot ≤ x /\ pivot <> x;
+          forall x : A, In x hi -> R pivot x /\ pivot <> x;
     len_lo :
       forall (pivot : A) (l lo eq hi : list A),
         partition pivot l = (lo, eq, hi) ->
@@ -53,7 +53,7 @@ Class Partition (A : LinDec) : Type :=
     partition_perm :
       forall (pivot : A) (l lo eq hi : list A),
         partition pivot l = (lo, eq, hi) ->
-          perm A l (lo ++ eq ++ hi);
+          Permutation l (lo ++ eq ++ hi);
 }.
 
 Coercion partition : Partition >-> Funclass.
@@ -61,24 +61,24 @@ Coercion partition : Partition >-> Funclass.
 (* Lemmas about [sorted]. *)
 
 Theorem sorted_tail :
-  forall (A : LinDec) (h : A) (t : list A),
-    sorted A (h :: t) -> sorted A t.
+  forall (A : Type) (R : A -> A -> Prop) (h : A) (t : list A),
+    sorted R (h :: t) -> sorted R t.
 Proof.
   inversion 1; auto.
 Defined.
 
 Theorem sorted_head :
-  forall (A : LinDec) (x y : A) (l : list A),
-    sorted A (x :: y :: l) -> x ≤ y.
+  forall (A : Type) (R : A -> A -> Prop) (x y : A) (l : list A),
+    sorted R (x :: y :: l) -> R x y.
 Proof.
   inversion 1. assumption.
 Qed.
 
 Lemma sorted_app_all :
-  forall (A : LinDec) (l : list A) (h : A) (t : list A),
-    sorted A l -> sorted A (h :: t) ->
-    (forall x : A, In x l -> leq x h) ->
-      sorted A (l ++ h :: t).
+  forall (A : Type) (R : A -> A -> Prop) (l : list A) (h : A) (t : list A),
+    sorted R l -> sorted R (h :: t) ->
+    (forall x : A, In x l -> R x h) ->
+      sorted R (l ++ h :: t).
 Proof.
   induction l as [| h t]; simpl; intros.
     assumption.
@@ -95,21 +95,21 @@ Proof.
 Qed.
 
 Lemma sorted_app :
-  forall (A : LinDec) (l1 l2 : list A),
-    sorted A l1 -> sorted A l2 ->
-      (forall x y : A, In x l1 -> In y l2 -> x ≤ y) ->
-        sorted A (l1 ++ l2).
+  forall (A : Type) (R : A -> A -> Prop) (l1 l2 : list A),
+    sorted R l1 -> sorted R l2 ->
+      (forall x y : A, In x l1 -> In y l2 -> R x y) ->
+        sorted R (l1 ++ l2).
 Proof.
   destruct l2 as [| h2 t2]; cbn; intros.
     rewrite app_nil_r. assumption.
     apply sorted_app_all; auto.
 Qed.
 
-Hint Resolve sorted_head sorted_tail sorted_app_all.
+Hint Resolve (*sorted_head*) sorted_tail sorted_app_all.
 
 Lemma sorted_cons :
-  forall (A : LinDec) (h : A) (t : list A),
-    (forall x : A, In x t -> h ≤ x) -> sorted A t -> sorted A (h :: t).
+  forall (A : Type) (R : A -> A -> Prop) (h : A) (t : list A),
+    (forall x : A, In x t -> R h x) -> sorted R t -> sorted R (h :: t).
 Proof.
   inversion 2; subst.
     auto.
@@ -120,43 +120,42 @@ Proof.
 Qed.
 
 Lemma sorted_mid :
-  forall (A : LinDec) (x y : A) (l : list A),
-    sorted A (x :: y :: l) -> sorted A (x :: l).
+  forall (A : Type) (R : A -> A -> Prop) (x y : A) (l : list A)
+    (R_trans : forall x y z : A, R x y -> R y z -> R x z),
+      sorted R (x :: y :: l) -> sorted R (x :: l).
 Proof.
   destruct l.
     auto.
     intros. constructor.
-      assert (x ≤ y) by (apply sorted_head in H; auto).
+      assert (R x y) by (apply sorted_head in H; auto).
         apply sorted_tail in H.
-        assert (y ≤ c) by (apply sorted_head in H; auto).
-        eapply leq_trans; eauto.
+        assert (R y a) by (apply sorted_head in H; auto).
+        eapply R_trans; eauto.
       do 2 eapply sorted_tail. eassumption.
 Qed.
 
 Lemma sorted_cons_conv :
-  forall (A : LinDec) (h : A) (t : list A),
-    sorted A (h :: t) -> forall x : A, In x t -> h ≤ x.
+  forall (A : Type) (R : A -> A -> Prop) (h : A) (t : list A)
+    (R_trans : forall x y z : A, R x y -> R y z -> R x z),
+    sorted R (h :: t) -> forall x : A, In x t -> R h x.
 Proof.
-  induction t as [| h' t'].
-    inversion 2.
-    intros. inversion H0; subst.
-      apply sorted_head in H. assumption.
-      apply IHt'.
-        apply sorted_mid in H. assumption.
-        assumption.
+  induction t as [| h' t']; inv 3.
+    apply sorted_head with t'. assumption.
+    apply IHt'; try assumption.
+      apply sorted_mid with h'; assumption.
 Qed.
 
 Lemma sorted_cons_conv' :
-  forall (A : LinDec) (h : A) (t : list A),
-    sorted A (h :: t) -> forall x : A, In x (h :: t) -> h ≤ x.
+  forall (A : Type) (R : A -> A -> Prop) (h : A) (t : list A)
+    (R_refl : forall x : A, R x x)
+    (R_trans : forall x y z : A, R x y -> R y z -> R x z),
+      sorted R (h :: t) -> forall x : A, In x (h :: t) -> R h x.
 Proof.
-  induction t as [| h' t'].
-    inversion 2; subst; dec.
-    do 2 inversion 1; subst.
-      dec.
-      inversion H6; subst.
-        assumption.
-        apply IHt'.
-          eapply sorted_mid; eauto.
-          right. assumption.
+  induction t as [| h' t']; inv 4.
+    inv H1.
+    inv H1.
+      inv H.
+      apply IHt'; try assumption.
+        apply sorted_mid with h'; assumption.
+        right. assumption.
 Qed.
