Sorting/Perm_generalizd.v
@@ -1,0 +1,335 @@
+Add Rec LoadPath "/home/zeimer/Code/Coq".
+
+Require Export RCCBase.
+
+Require Export LinDec.
+
+Require Export Sorting.ListLemmas.
+Require Import TrichDec.
+
+Require Import Classes.RelationClasses.
+Require Import Permutation.
+
+Fixpoint count {A : Type} (p : A -> bool) (l : list A) : nat :=
+match l with
+    | [] => 0
+    | h :: t => if p h then S (count p t) else count p t
+end.
+
+Definition perm {A : Type} (l1 l2 : list A) : Prop :=
+  forall p : A -> bool, count p l1 = count p l2.
+
+(* Lemmas about [count]. *)
+
+Lemma count_app :
+  forall (A : Type) (p : A -> bool) (l1 l2 : list A),
+    count p (l1 ++ l2) = count p l1 + count p l2.
+Proof.
+  induction l1; cbn; intros.
+    reflexivity.
+    rewrite IHl1. destruct (p a); cbn; reflexivity.
+Qed.
+
+Lemma count_app_comm :
+  forall (A : Type) (p : A -> bool) (l1 l2 : list A),
+    count p (l1 ++ l2) = count p (l2 ++ l1).
+Proof.
+  induction l1 as [| h1 t1]; cbn; intros.
+    rewrite app_nil_r. reflexivity.
+    rewrite !count_app. cbn. destruct (p h1); omega.
+Qed.
+
+Lemma count_last :
+  forall (A : Type) (p : A -> bool) (l : list A) (x : A),
+    count p (l ++ [x]) = count p l + count p [x].
+Proof.
+  intros. rewrite count_app. reflexivity.
+Qed.
+
+Lemma count_reverse :
+  forall (A : Type) (p : A -> bool) (l : list A),
+    count p (rev l) = count p l.
+Proof.
+  induction l as [| h t]; cbn; intros.
+    reflexivity.
+    rewrite count_app, IHt. cbn. destruct (p h); omega.
+Qed.
+
+Lemma count_cons :
+  forall (A : Type) (p : A -> bool) (h : A) (t : list A),
+    p h = true -> count p (h :: t) = 1 + count p t.
+Proof.
+  intros. cbn. rewrite H. reflexivity.
+Qed.
+
+Lemma count_filter :
+  forall (A : Type) (p : A -> bool) (t : list A),
+    count p t = count p (filter p t) +
+                count p (filter (fun x : A => negb (p x)) t).
+Proof.
+  induction t as [| h' t']; cbn.
+    reflexivity.
+    destruct (p h') eqn: H; cbn; rewrite ?H, ?IHt'; reflexivity.
+Qed.
+
+Lemma count_In :
+  forall (A : Type) (p : A -> bool) (l : list A),
+    Exists (fun x => p x = true) l <-> count p l <> 0.
+Proof.
+  split.
+    induction 1; cbn.
+      rewrite H. inv 1.
+      destruct (p x).
+        inv 1.
+        assumption.
+    induction l as [| h t]; cbn; intros.
+      contradiction.
+      destruct (p h) eqn: Hph.
+        left. assumption.
+        right. apply IHt, H.
+Qed.
+
+(*Lemma count_0_nil :
+  forall (A : Type) (l : list A),
+    (forall p : A -> bool, count p l = 0) -> l = [].
+Proof.
+  induction l as [| h t]; cbn; intros.
+    trivial.
+    specialize (H h). dec.
+Qed.*)
+
+(* Lemmas about [perm]. *)
+Lemma perm_refl :
+  forall (A : Type) (l : list A), perm l l.
+Proof. unfold perm; auto. Defined.
+
+Lemma perm_sym :
+  forall (A : Type) (l1 l2 : list A),
+    perm l1 l2 -> perm l2 l1.
+Proof. unfold perm; auto. Defined.
+
+Lemma perm_trans :
+  forall (A : Type) (l1 l2 l3 : list A),
+    perm l1 l2 -> perm l2 l3 -> perm l1 l3.
+Proof.
+  unfold perm; intros. eapply eq_trans; auto.
+Defined.
+
+Hint Resolve perm_refl perm_sym.
+
+Instance Equiv_perm (A : Type) : Equivalence (@perm A).
+Proof.
+  split; red; intros; eauto. eapply perm_trans; eauto.
+Defined.
+
+Lemma perm_cons :
+  forall (A : Type) (x : A) (l1 l2 : list A),
+    perm l1 l2 -> perm (x :: l1) (x :: l2).
+Proof.
+  unfold perm. intros. cbn. rewrite H. reflexivity.
+Defined.
+
+Lemma perm_nil_cons :
+  forall (A : Type) (h : A) (t : list A),
+    ~ perm (h :: t) [].
+Proof.
+  unfold not; intros. red in H.
+  specialize (H (fun _ => true)).
+  cbn in H. inv H.
+Qed.
+
+Lemma perm_swap :
+  forall (A : Type) (x y : A) (l1 l2 : list A),
+    perm l1 l2 -> perm (x :: y :: l1) (y :: x :: l2).
+Proof.
+  unfold perm; cbn; intros; destruct (p x), (p y);
+  rewrite H; auto.
+Defined.
+
+Theorem perm_front :
+  forall (A : Type) (x : A) (l1 l2 : list A),
+    perm (l1 ++ x :: l2) (x :: l1 ++ l2).
+Proof.
+  induction l1 as [| h1 t1]; simpl; intros.
+    apply perm_refl.
+    eapply perm_trans with (h1 :: x :: t1 ++ l2).
+      apply perm_cons. apply IHt1.
+      apply perm_swap. apply perm_refl.
+Qed.
+
+Hint Resolve perm_refl perm_sym perm_cons perm_swap perm_front.
+
+Lemma perm_app_comm :
+  forall (A : Type) (l1 l2 : list A),
+    perm (l1 ++ l2) (l2 ++ l1).
+Proof.
+  unfold perm. intros. apply count_app_comm.
+Qed.
+
+Lemma perm_app :
+  forall (A : Type) (l1 l1' l2 l2' : list A),
+    perm l1 l1' -> perm l2 l2' -> perm (l1 ++ l2) (l1' ++ l2').
+Proof.
+  unfold perm; intros. rewrite 2 count_app, H, H0. auto.
+Qed.
+
+Require Import ListLemmas_generalized.
+
+Lemma perm_In :
+  forall (A : Type) (P : A -> Prop) (l l' : list A),
+    Exists P l -> perm l l' -> Exists P l'.
+Proof.
+  induction 1; intro.
+    destruct l'.
+      apply perm_nil_cons in H0. contradiction.
+      red in H0. cbn in H0. specialize (H0 p). rewrite H in H0.
+          destruct (p a) eqn: Ha.
+            left. assumption.
+            right.
+
+(* TODO: zostawić count, ale cofnąć perm *)
+Abort. (*
+
+rewrite count_In. red in H0. rewrite <- H0.
+  rewrite <- count_In. assumption.
+Qed.
+
+Lemma perm_singl :
+  forall (A : Type) (p : A -> bool) (l : list A),
+    perm [x] l -> l = [x].
+Proof.
+  unfold perm; destruct l as [| h1 [| h2 t]]; cbn; intros.
+    specialize (H x). dec.
+    specialize (H x). dec.
+    assert (H1 := H h1). assert (H2 := H h2). dec.
+Qed.
+
+Lemma perm_cons_inv :
+  forall (A : Type) (h : A) (t1 t2 : list A),
+    perm (h :: t1) (h :: t2) -> perm t1 t2.
+Proof.
+  unfold perm; intros. specialize (H x). cbn in H. dec.
+Qed.
+
+Lemma removeFirst_In_perm :
+  forall (A : Type) (p : A -> bool) (l : list A),
+    In x l -> perm l (x :: removeFirst x l).
+Proof.
+  induction l as [| h t]; cbn; inv 1; dec.
+    specialize (IHt H0). rewrite <- perm_swap.
+      apply perm_cons. exact IHt.
+      reflexivity.
+Qed.
+
+Lemma perm_In' :
+  forall (A : Type) (h : A) (t l : list A),
+    perm (h :: t) l -> In h l.
+Proof.
+  intros. rewrite count_In. rewrite <- H. cbn. dec.
+Defined.
+
+Lemma count_removeFirst_neq :
+  forall (A : Type) (x y : A) (l : list A),
+    x <> y -> count p (removeFirst y l) = count p l.
+Proof.
+  induction l as [| h t]; cbn; intros; dec; dec.
+Qed.
+
+Lemma count_removeFirst_In :
+  forall (A : Type) (p : A -> bool) (l : list A),
+    In x l -> count p (removeFirst x l) = count p l - 1.
+Proof.
+  induction l as [| h t]; cbn; intros.
+    reflexivity.
+    firstorder (repeat dec).
+Qed.
+
+Lemma perm_removeFirst :
+  forall (A : Type) (h h' : A) (t t' : list A),
+    h <> h' -> perm (h :: t) (h' :: t') ->
+      perm (h :: removeFirst h' t) t'.
+Proof.
+  intros. assert (In h' t).
+    symmetry in H0. apply perm_In' in H0. cbn in H0. destruct H0.
+      congruence.
+      assumption.
+    unfold perm. intro. destruct (x =? h) eqn: Heq; dec.
+      rewrite count_removeFirst_neq.
+        red in H0. specialize (H0 h). cbn in H0. dec.
+        assumption.
+      destruct (x =? h') eqn: Heq'; dec.
+        rewrite count_removeFirst_In.
+          red in H0. specialize (H0 h'). cbn in H0. dec.
+          assumption.
+        rewrite count_removeFirst_neq.
+          red in H0. specialize (H0 x). cbn in H0. dec.
+          assumption.
+Qed.
+
+Lemma perm_front_ex' :
+  forall (A : Type) (h : A) (t l : list A),
+    perm (h :: t) l -> exists l1 l2 : list A,
+      l = l1 ++ h :: l2 /\ perm (l1 ++ l2) t.
+Proof.
+  intros A h t l. gen t; gen h.
+  induction l as [| h' t']; cbn; intros.
+    apply perm_nil_cons in H. contradiction.
+    destruct (h =? h') eqn: Heq.
+      dec. exists [], t'. cbn. split.
+        reflexivity.
+        apply perm_cons_inv in H. rewrite H. reflexivity.
+      dec. assert (perm (h :: removeFirst h' t) t').
+        apply perm_removeFirst; assumption.
+        destruct (IHt' h (removeFirst h' t) H0) as (l1 & l2 & H1 & H2).
+          clear IHt'. subst. exists (h' :: l1), l2. split.
+            reflexivity.
+            cbn. rewrite (removeFirst_In_perm h' t).
+              apply perm_cons. assumption.
+              rewrite app_comm_cons, perm_app_comm in H; cbn in H.
+                apply perm_cons_inv in H. eapply perm_In.
+                  Focus 2. rewrite H. reflexivity.
+                  apply in_or_app. right. left. reflexivity.
+Qed.
+
+Theorem Permutation_perm :
+  forall (A : Type) (l1 l2 : list A),
+    Permutation l1 l2 -> perm l1 l2.
+Proof.
+  induction 1; cbn; intros; dec.
+Qed.
+
+Theorem perm_Permutation :
+  forall (A : Type) (l1 l2 : list A),
+    perm l1 l2 -> Permutation l1 l2.
+Proof.
+  induction l1 as [| h1 t1]; cbn; intros.
+    destruct l2; cbn; auto. red in H. cbn in H. specialize (H c). dec.
+    apply perm_front_ex' in H. destruct H as (l1 & l3 & H1 & H3). subst.
+      rewrite <- Permutation_cons_app.
+        reflexivity.
+        apply IHt1. symmetry. assumption.
+Qed.
+
+(** Moved from ListLemmas to avoid circularity. *)
+
+Lemma perm_min_front :
+  forall (A : Type) (h : A) (t : list A),
+    let m := min_dflt A h t in
+      perm (m :: removeFirst m (h :: t)) (h :: t).
+Proof.
+  intros. destruct (min_split A h t) as [l1 [l2 [H H']]]. fold m in H, H'.
+  rewrite H, <- H' in *. apply perm_symm. apply perm_front.
+Qed.
+
+Theorem trifilter_spec' :
+  forall (A : TrichDec) (pivot : A) (l lo eq hi : list A),
+    trifilter pivot l = (lo, eq, hi) ->
+      perm (lo ++ eq) (filter (fun x : A => x <=? pivot) l) /\
+      hi = filter (fun x : A => pivot <? x) l.
+Proof.
+  intros until hi. functional induction trifilter pivot l;
+  intros; inv H; cbn in *; trich; edestruct IHp; try split; eauto.
+    apply perm_cons; auto.
+    rewrite (perm_front A x lo l2). apply perm_cons. auto.
+    f_equal. auto.
+Qed.*)
